Everything parses now

src/Interpreter.fst
@@ -19,14 +19,14 @@ open Total
    assignment. *)
 
 (* A representation of program heap (which is Bool-typed) *)
-type interpretation (state:Type) =
+noeq type interpretation (state:eqtype) =
   { alloc  : state -> Tot (int * state);
-    assign : state -> int -> BoolExp -> Tot state;
+    assign : state -> int -> boolExp -> Tot state;
     eval   : state -> Total.state -> int -> Tot bool }
 
 (* Values of the language *)
-val isVal : gexp:GExpr -> Tot bool (decreases %[gexp;1])
-val isVal_lst : lst:list GExpr -> Tot bool (decreases %[lst;0])
+val isVal : gexp:gExpr -> Tot bool (decreases %[gexp;1])
+val isVal_lst : lst:list gExpr -> Tot bool (decreases %[lst;0])
 let rec isVal tm = match tm with
   | UNIT          -> true
   | LAMBDA (s, ty, t) -> true
@@ -38,32 +38,32 @@ and isVal_lst lst = match lst with
   | (LOC l)::xs -> isVal_lst xs
   | _ -> false
 
-val isBexp : GExpr -> Tot bool
+val isBexp : gExpr -> Tot bool
 let isBexp tm = match tm with
   | LOC i     -> true
   | BEXP bexp -> true
   | BOOL b    -> true
   | _         -> false
 
-type config     (state:Type) = GExpr * state
+type config     (state:Type) = gExpr * state
 type valconfig  (state:Type) = c:(config state){isVal (fst c)}
-type listconfig (state:Type) = (list GExpr) * state
+type listconfig (state:Type) = (list gExpr) * state
 
-val get_bexp : gexp:GExpr{isBexp gexp} -> Tot BoolExp
+val get_bexp : gexp:gExpr{isBexp gexp} -> Tot boolExp
 let get_bexp gexp = match gexp with
   | LOC i     -> BVar i
   | BEXP bexp -> bexp
   | BOOL b    -> if b then BNot BFalse else BFalse
 
 (* Small-step evaluator *)
-val step : #state:Type -> c:config state -> interpretation state ->
+val step : #state:eqtype -> c:config state -> interpretation state ->
   Tot (result (config state)) (decreases %[(fst c);1])
-val step_lst : #state:Type -> c:listconfig state -> interpretation state ->
+val step_lst : #state:eqtype -> c:listconfig state -> interpretation state ->
   Tot (result (listconfig state)) (decreases %[(fst c);0])
-let rec step (tm, st) interp = match tm with
+let rec step #s (tm, st) interp = match tm with
   | LET (x, t1, t2) ->
     if isVal t1
-    then Val (substGExpr t2 x t1, st)
+    then Val (substgExpr t2 x t1, st)
     else bindT (step (t1, st) interp) (fun (t1', st') -> Val (LET (x, t1', t2), st'))
   | APPLY (t1, t2) ->
     if not (isVal t1) then
@@ -72,7 +72,7 @@ let rec step (tm, st) interp = match tm with
       bindT (step (t2, st) interp) (fun (t2', st') -> Val (APPLY (t1, t2'), st'))
     else
       begin match t1 with
-        | LAMBDA (x, ty, t) -> Val (substGExpr t x t2, st)
+        | LAMBDA (x, ty, t) -> Val (substgExpr t x t2, st)
         | _ -> Err (String.strcat "Cannot reduce application: " (show tm))
       end
   | SEQUENCE (t1, t2) ->
@@ -126,7 +126,7 @@ let rec step (tm, st) interp = match tm with
     else
       begin match t with
         | ARRAY lst ->
-          if (0 <= i && i < List.lengthT lst) then
+          if (0 <= i && i < FStar.List.Tot.length lst) then
             Val (ARRAY (rotate lst i), st)
           else
             Err (String.strcat "Array out of bounds: " (show tm))
@@ -138,21 +138,28 @@ let rec step (tm, st) interp = match tm with
     else
       begin match t with
         | ARRAY lst ->
-          if (0 <= i && i <= j && j < List.lengthT lst) then
+          if (0 <= i && i <= j && j < FStar.List.Tot.length lst) then
             Val (ARRAY (slice lst i j), st)
           else
             Err (String.strcat "Array out of bounds: " (show tm))
         | _ -> Err (String.strcat "Cannot reduce slice: " (show tm))
       end
-  | ARRAY lst ->
-    bindT (step_lst (lst, st) interp) (fun (lst, st') -> Val (ARRAY lst, st'))
+  | ARRAY lst -> admit()
+    (* NOTE: fix this eventually. In the old version of F* this worked
+         bindT (step_lst (lst, st) (fun c -> step c interp)) (fun (lst, st') -> Val (ARRAY lst, st'))
+       However, with decidable and propositional equality now in F*, the interpretation type
+       doesn't support decidable type equality in general, so F* fails to type check the mutual
+       recursive application here. Can't find another solution that works -- local definitions
+       don't appear to support totality proofs or for that matter mutual recursion, and I can't get
+       F* to infer that the x in ARRAY (x::xs) is a subterm so direct recursion is out. It'll have to
+       be left like this until I can get some help from the dev team *)
   | GET_ARRAY (t, i) ->
     if not (isVal t) then
       bindT (step (t, st) interp) (fun (t', st') -> Val (GET_ARRAY (t', i), st'))
     else
       begin match t with
         | ARRAY lst ->
-          if (0 <= i && i < List.lengthT lst) then
+          if (0 <= i && i < FStar.List.Tot.length lst) then
             Val (nthT lst i, st)
           else
             Err (String.strcat "Array out of bounds: " (show tm))
@@ -171,27 +178,29 @@ let rec step (tm, st) interp = match tm with
     let st''     = interp.assign st' l (BXor (BVar l, bexp)) in
       Val (LOC l, st'')
   | _ -> Err (String.strcat "No rule applies: " (show tm))
-and step_lst (lst, st) interp = match lst with
+and step_lst #s (lst, st) interp = match lst with
   | [] -> Val ([], st)
   | x::xs ->
-    if not (isVal x) then
-      bindT (step (x, st) interp) (fun (x', st') -> Val (x'::xs, st'))
+    if not (isVal x) then admit()
+      (* See note above
+           bindT (step (x, st) interp) (fun (x', st') -> Val (x'::xs, st')) *)
     else
       bindT (step_lst (xs, st) interp) (fun (xs', st') -> Val (x::xs', st'))
 
 (* Big-step evaluator. More efficient but not (proven) total *)
-val eval_rec : #state:Type -> config state -> interpretation state -> result (config state)
-val eval_to_bexp : #state:Type -> config state -> interpretation state -> result (config state)
-let rec eval_rec (tm, st) interp = match tm with
+(* NOTE: commented out due to decidable equality issues as above. Not currently used anyway
+val eval_rec : #state:eqtype -> config state -> interpretation state -> result (config state)
+val eval_to_bexp : #state:eqtype -> config state -> interpretation state -> result (config state)
+let rec eval_rec #s (tm, st) interp = match tm with
   | LET (x, t1, t2) ->
     bind (eval_rec (t1, st) interp) (fun (v1, st') ->
-      eval_rec (substGExpr t2 x v1, st') interp)
+      eval_rec (substgExpr t2 x v1, st') interp)
   | LAMBDA (x, ty, t) -> Val (tm, st)
   | APPLY (t1, t2) ->
     bind (eval_rec (t1, st) interp)  (fun (v1, st') ->
     bind (eval_rec (t2, st') interp) (fun (v2, st'') ->
     begin match v1 with
-      | LAMBDA (x, ty, t) -> eval_rec (substGExpr t x v2, st'') interp
+      | LAMBDA (x, ty, t) -> eval_rec (substgExpr t x v2, st'') interp
       | _ -> Err (String.strcat "LHS is not a lambda: " (show tm))
     end))
   | SEQUENCE (t1, t2) ->
@@ -217,7 +226,7 @@ let rec eval_rec (tm, st) interp = match tm with
     bind (eval_rec (t, st) interp) (fun (v, st') ->
     begin match v with
       | ARRAY lst ->
-        if (0 <= i && i < List.length lst)
+        if (0 <= i && i < FStar.List.Tot.length lst)
         then Val (ARRAY (rotate lst i), st')
         else Err (String.strcat "Rotation out of array bounds: " (show tm))
       | _ -> Err (String.strcat "Rotation of non-array argument: " (show tm))
@@ -226,7 +235,7 @@ let rec eval_rec (tm, st) interp = match tm with
     bind (eval_rec (t, st) interp) (fun (v, st') ->
     begin match v with
       | ARRAY lst ->
-        if (0 <= i && i <= j && j < List.length lst)
+        if (0 <= i && i <= j && j < FStar.List.Tot.length lst)
         then Val (ARRAY (slice lst i j), st')
         else Err (String.strcat "Invalid slice bounds: " (show tm))
       | _ -> Err (String.strcat "Slice of non-array argument: " (show tm))
@@ -240,13 +249,13 @@ let rec eval_rec (tm, st) interp = match tm with
       end)
     in
     bind (foldM f ([], st) tlst) (fun (llst, st') ->
-      Val (ARRAY (List.rev llst), st'))
+      Val (ARRAY (FStar.List.Tot.rev llst), st'))
   | GET_ARRAY (t, i) ->
     bind (eval_rec (t, st) interp) (fun (v, st') ->
     begin match v with
       | ARRAY lst ->
-        if (0 <= i && i < List.length lst) then
-          match List.total_nth lst i with
+        if (0 <= i && i < FStar.List.Tot.length lst) then
+          match FStar.List.Tot.nth lst i with
             | Some (LOC l) -> Val (LOC l, st')
             | Some _ -> Err ("Impossible")
             | None -> Err (String.strcat "Array out of bounds: " (show tm))
@@ -265,7 +274,7 @@ let rec eval_rec (tm, st) interp = match tm with
     let st''     = interp.assign st l (BXor (BVar l, bexp)) in
       Val (LOC l, st')
   | _ -> Err (String.strcat "Unimplemented case: " (show tm))
-and eval_to_bexp (tm, st) interp = match tm with
+and eval_to_bexp #s (tm, st) interp = match tm with
   | XOR (x, y) ->
     bind (eval_to_bexp (x, st) interp)  (fun (x', st') ->
     bind (eval_to_bexp (y, st') interp) (fun (y', st'') ->
@@ -285,6 +294,7 @@ and eval_to_bexp (tm, st) interp = match tm with
     match v with
       | LOC l -> Val (BEXP (BVar l), st')
       | _ -> Err (String.strcat "Could not reduce expression to boolean: " (show tm)))
+*)
 
 (** Interpretation domains *)
 
@@ -293,7 +303,7 @@ type boolState = int * (Total.t int bool)
 
 val boolInit   : boolState
 val boolAlloc  : boolState -> Tot (int * boolState)
-val boolAssign : boolState -> int -> BoolExp -> Tot boolState
+val boolAssign : boolState -> int -> boolExp -> Tot boolState
 val boolEval   : boolState -> state -> int -> Tot bool
 
 let boolInit = (0, constMap false)
@@ -307,8 +317,8 @@ let boolInterp = {
   eval = boolEval
 }
 
-val substVal : v:GExpr{isVal v} -> st:boolState -> Tot GExpr
-val substVal_lst : v:(list GExpr){isVal_lst v} -> st:boolState -> Tot (list GExpr)
+val substVal : v:gExpr{isVal v} -> st:boolState -> Tot gExpr
+val substVal_lst : v:(list gExpr){isVal_lst v} -> st:boolState -> Tot (list gExpr)
 let rec substVal v st = match v with
   | UNIT | LAMBDA _ -> v
   | LOC l -> BOOL (lookup (snd st) l)
@@ -328,27 +338,27 @@ let eval gexp = evalBool (gexp, boolInit)
 (** Verification utilities *)
 
 type alloc_preservation 
-  (#s1:Type) 
-  (#s2:Type) 
+  (#s1:eqtype) 
+  (#s2:eqtype) 
   (i1:interpretation s1) 
   (i2:interpretation s2) 
   (p:s1 -> s2 -> Total.t int bool -> Type) =
     forall st1 st2 init. p st1 st2 init ==> p (snd (i1.alloc st1)) (snd (i2.alloc st2)) init
 
 type assign_preservation 
-  (#s1:Type) 
-  (#s2:Type) 
+  (#s1:eqtype) 
+  (#s2:eqtype) 
   (i1:interpretation s1) 
   (i2:interpretation s2) 
   (p:s1 -> s2 -> Total.t int bool -> Type) =
     forall st1 st2 i bexp init. p st1 st2 init ==> p (i1.assign st1 i bexp) (i2.assign st2 i bexp) init
 
 val step_preservation : 
-  #s1:Type -> #s2:Type -> i1:interpretation s1 -> i2:interpretation s2 ->
+  #s1:eqtype -> #s2:eqtype -> i1:interpretation s1 -> i2:interpretation s2 ->
   p:(s1 -> s2 -> Total.t int bool -> Type) ->
   h1:alloc_preservation i1 i2 p ->
   h2:assign_preservation i1 i2 p ->
-  gexp:GExpr -> st1:s1 -> st2:s2 -> init:Total.t int bool ->
+  gexp:gExpr -> st1:s1 -> st2:s2 -> init:Total.t int bool ->
   Lemma (requires (p st1 st2 init))
         (ensures
           (is_Err (step (gexp, st1) i1) /\ is_Err (step (gexp, st2) i2)) \/
@@ -356,11 +366,11 @@ val step_preservation :
 	    p (snd (getVal (step (gexp, st1) i1))) (snd (getVal (step (gexp, st2) i2))) init))
   (decreases %[gexp;1])
 val step_preservation_lst : 
-  #s1:Type -> #s2:Type -> i1:interpretation s1 -> i2:interpretation s2 ->
+  #s1:eqtype -> #s2:eqtype -> i1:interpretation s1 -> i2:interpretation s2 ->
   p:(s1 -> s2 -> Total.t int bool -> Type) ->
   h1:alloc_preservation i1 i2 p ->
   h2:assign_preservation i1 i2 p ->
-  lst:list GExpr -> st1:s1 -> st2:s2 -> init:Total.t int bool ->
+  lst:list gExpr -> st1:s1 -> st2:s2 -> init:Total.t int bool ->
   Lemma (requires (p st1 st2 init))
         (ensures
           (is_Err (step_lst (lst, st1) i1) /\ is_Err (step_lst (lst, st2) i2)) \/
@@ -368,50 +378,48 @@ val step_preservation_lst :
 	    p (snd (getVal (step_lst (lst, st1) i1))) (snd (getVal (step_lst (lst, st2) i2))) init))
   (decreases %[lst;0])
 
-(* F* compiler complains this is not total, no idea what's happening
-let rec step_preservation i1 i2 p h1 h2 gexp st1 st2 init = admit () (*match gexp with
-  | LET (x, t1, t2) -> admit() //step_preservation i1 i2 p h1 h2 t1 st1 st2 init
+(* F* compiler complains this is not total, no idea what's happening *)
+let rec step_preservation #s1 #s2 i1 i2 p h1 h2 gexp st1 st2 init = match gexp with
+  | LET (x, t1, t2) -> step_preservation i1 i2 p h1 h2 t1 st1 st2 init
   | LAMBDA (x, ty, t) -> ()
-  | APPLY (t1, t2) ->
-    state_equiv_step t1 st st' init;
-    state_equiv_step t2 st st' init
+  | APPLY (t1, t2) -> 
+    step_preservation i1 i2 p h1 h2 t1 st1 st2 init;
+    step_preservation i1 i2 p h1 h2 t2 st1 st2 init
   | SEQUENCE (t1, t2) ->
-    state_equiv_step t1 st st' init
+    step_preservation i1 i2 p h1 h2 t1 st1 st2 init;
+    step_preservation i1 i2 p h1 h2 t2 st1 st2 init
   | ASSIGN (t1, t2) ->
-    state_equiv_step t1 st st' init;
-    state_equiv_step t2 st st' init;
+    step_preservation i1 i2 p h1 h2 t1 st1 st2 init;
+    step_preservation i1 i2 p h1 h2 t2 st1 st2 init;
     if (isVal t1 && isBexp t2) then
       begin match t1 with
-        | LOC l -> state_equiv_assign st st' init l (get_bexp t2)
+        | LOC l -> admit() //h2
         | _ -> ()
-      end
+      end (*
   | XOR (t1, t2) ->
-    state_equiv_step t1 st st' init;
-    state_equiv_step t2 st st' init
+    step_preservation i1 i2 p h1 h2 t1 st1 st2 init;
+    step_preservation i1 i2 p h1 h2 t2 st1 st2 init
   | AND (t1, t2) ->
-    state_equiv_step t1 st st' init;
-    state_equiv_step t2 st st' init
+    step_preservation i1 i2 p h1 h2 t1 st1 st2 init;
+    step_preservation i1 i2 p h1 h2 t2 st1 st2 init
   | BOOL b -> ()
-  | APPEND (t1, t2) ->
-    state_equiv_step t1 st st' init;
-    state_equiv_step t2 st st' init
+  | APPEND (t1, t2) -> ()
+    step_preservation i1 i2 p h1 h2 t1 st1 st2 init;
+    step_preservation i1 i2 p h1 h2 t2 st1 st2 init;
   | ROT (i, t) ->
     state_equiv_step t st st' init
   | SLICE (t, i, j) ->
     state_equiv_step t st st' init
-  | ARRAY lst ->
-    state_equiv_step_lst lst st st' init
+  | ARRAY lst -> admit()
+    //state_equiv_step_lst lst st st' init
   | GET_ARRAY (t, i) ->
     state_equiv_step t st st' init
   | ASSERT t ->
     state_equiv_step t st st' init
-  | BEXP bexp -> state_equiv_alloc st st' init bexp
-  | _ -> ()
-and step_preservation_lst i1 i2 p h1 h2 gexp st1 st2 init = admit() (*match lst with
+  | BEXP bexp -> state_equiv_alloc st st' init bexp *)
+  | _ -> admit()
+and step_preservation_lst #s1 #s2 i1 i2 p h1 h2 gexp st1 st2 init = admit() (*match lst with
   | [] -> ()
   | x::xs ->
     state_equiv_step x st st' init;
-    state_equiv_step_lst xs st st' init
-*)
-*)
-*)
+    state_equiv_step_lst xs st st' init *)
